wip: fixed window scalar multiplication for ed25519

lib/Lib.NatMod.fsti
@@ -2,6 +2,9 @@ module Lib.NatMod
 
 open FStar.Mul
 
+module Fermat = FStar.Math.Fermat
+module Euclid = FStar.Math.Euclid
+
 module LE = Lib.Exponentiation
 
 #set-options "--z3rlimit 10 --fuel 0 --ifuel 0"
@@ -28,6 +31,8 @@ val lemma_pow_ge_zero: a:nat -> b:nat -> Lemma (pow a b >= 0) [SMTPat (pow a b)]
 
 val lemma_pow_nat_is_pow: a:int -> b:nat ->
   Lemma (pow a b == LE.pow mk_nat_comm_monoid a b)
+
+val lemma_pow_one: b:nat -> Lemma (pow 1 b = 1)
 
 val lemma_pow_add: x:int -> n:nat -> m:nat -> Lemma (pow x n * pow x m = pow x (n + m))
 
@@ -68,3 +73,36 @@ val lemma_pow_mod: #m:pos{1 < m} -> a:nat_mod m -> b:nat -> Lemma (pow a b % m =
 
 val lemma_pow_nat_mod_is_pow: #n:pos{1 < n} -> a:nat_mod n -> b:nat ->
   Lemma (pow a b % n == LE.pow (mk_nat_mod_comm_monoid n) a b)
+
+
+let add_mod (#m:pos) (a:nat_mod m) (b:nat_mod m) : nat_mod m = (a + b) % m
+let sub_mod (#m:pos) (a:nat_mod m) (b:nat_mod m) : nat_mod m = (a - b) % m
+
+val lemma_mod_distributivity_add_right: #m:pos -> a:nat_mod m -> b:nat_mod m -> c:nat_mod m ->
+  Lemma (mul_mod a (add_mod b c) == add_mod (mul_mod a b) (mul_mod a c))
+
+val lemma_mod_distributivity_add_left: #m:pos -> a:nat_mod m -> b:nat_mod m -> c:nat_mod m ->
+  Lemma (mul_mod (add_mod a b) c == add_mod (mul_mod a c) (mul_mod b c))
+
+val lemma_mod_distributivity_sub_right: #m:pos -> a:nat_mod m -> b:nat_mod m -> c:nat_mod m ->
+  Lemma (mul_mod a (sub_mod b c) == sub_mod (mul_mod a b) (mul_mod a c))
+
+val lemma_mod_distributivity_sub_left: #m:pos -> a:nat_mod m -> b:nat_mod m -> c:nat_mod m ->
+  Lemma (mul_mod (sub_mod a b) c == sub_mod (mul_mod a c) (mul_mod b c))
+
+
+let prime = m:pos{1 < m /\ Euclid.is_prime m}
+let inv_mod (#m:prime) (a:nat_mod m) : nat_mod m = pow_mod #m a (m - 2)
+let div_mod (#m:prime) (a:nat_mod m) (b:nat_mod m) : nat_mod m = mul_mod a (inv_mod b)
+
+val lemma_inv_mod_both: #m:prime -> a:nat_mod m -> b:nat_mod m ->
+  Lemma (inv_mod (mul_mod a b) == mul_mod (inv_mod a) (inv_mod b))
+
+val lemma_div_mod_prime: #m:prime -> a:nat_mod m{a <> 0} -> Lemma (div_mod a a == 1)
+val lemma_div_mod_prime_one: #m:prime -> a:nat_mod m -> Lemma (div_mod a 1 == a)
+
+val lemma_div_mod_prime_cancel: #m:prime -> a:nat_mod m -> b:nat_mod m -> c:nat_mod m{c <> 0} ->
+  Lemma (div_mod (mul_mod a c) (mul_mod c b) == div_mod a b)
+
+val lemma_div_mod_prime_to_one_denominator: #m:prime -> a:nat_mod m -> b:nat_mod m -> c:nat_mod m{c <> 0} -> d:nat_mod m{d <> 0} ->
+  Lemma (mul_mod (div_mod a c) (div_mod b d) == div_mod (mul_mod a b) (mul_mod c d))
