specs/Spec.Ed25519.fst
@@ -4,134 +4,95 @@ open FStar.Mul
 open Lib.IntTypes
 open Lib.Sequence
 open Lib.ByteSequence
-open Lib.RawIntTypes
 
 open Spec.Curve25519
 
-#reset-options "--max_fuel 0 --z3rlimit 100"
+module LE = Lib.Exponentiation
+module SE = Spec.Exponentiation
+module EL = Spec.Ed25519.Lemmas
 
-///
-/// Constants
-///
+include Spec.Ed25519.PointOps
+
+#reset-options "--fuel 0 --ifuel 0 --z3rlimit 100"
 
 inline_for_extraction
 let size_signature: size_nat = 64
-
-
-type aff_point = elem & elem               // Affine point
-type ext_point = elem & elem & elem & elem // Homogeneous extended coordinates
-
-let modp_sqrt_m1 : elem = 2 **% ((prime - 1) / 4)
-
-let d : elem =
-  let x = 37095705934669439343138083508754565189542113879843219016388785533085940283555 in
-  assert_norm(x < prime);
-  x
 
 let q: n:nat{n < pow2 256} =
   assert_norm(pow2 252 + 27742317777372353535851937790883648493 < pow2 255 - 19);
   (pow2 252 + 27742317777372353535851937790883648493) // Group order
 
-let _:_:unit{Spec.Hash.Definitions.max_input_length Spec.Hash.Definitions.SHA2_512 > pow2 32} = assert_norm (Spec.Hash.Definitions.max_input_length Spec.Hash.Definitions.SHA2_512 > pow2 32)
-
-let g_x : elem = 15112221349535400772501151409588531511454012693041857206046113283949847762202
-let g_y : elem = 46316835694926478169428394003475163141307993866256225615783033603165251855960
-
-let g: ext_point = (g_x, g_y, 1, g_x *% g_y)
-
-///
-/// Internal functions
-///
-
-let modp_inv (x:elem) : Tot elem =
-  x **% (prime - 2)
+let _:_:unit{Spec.Hash.Definitions.max_input_length Spec.Hash.Definitions.SHA2_512 > pow2 32} =
+  assert_norm (Spec.Hash.Definitions.max_input_length Spec.Hash.Definitions.SHA2_512 > pow2 32)
 
 let sha512_modq (len:size_nat) (s:lbytes len) : n:nat{n < pow2 256} =
   nat_from_bytes_le (Spec.Agile.Hash.hash Spec.Hash.Definitions.SHA2_512 s) % q
 
-let point_add (p:ext_point) (q:ext_point) : Tot ext_point =
-  let x1, y1, z1, t1 = p in
-  let x2, y2, z2, t2 = q in
-  let a = (y1 -% x1) *% (y2 -% x2) in
-  let b = (y1 +% x1) *% (y2 +% x2) in
-  let c = (2 *% d *% t1) *% t2 in
-  let d = (2 *% z1) *% z2 in
-  let e = b -% a in
-  let f = d -% c in
-  let g = d +% c in
-  let h = b +% a in
-  let x3 = e *% f in
-  let y3 = g *% h in
-  let t3 = e *% h in
-  let z3 = f *% g in
-  (x3, y3, z3, t3)
+///  Point Multiplication
 
-let point_double (p:ext_point) : Tot ext_point =
-  let x1, y1, z1, t1 = p in
-  let a = x1 *% x1 in
-  let b = y1 *% y1 in
-  let c = 2 *% (z1 *% z1) in
-  let h = a +% b in
-  let e = h -% ((x1 +% y1) *% (x1 +% y1)) in
-  let g = a -% b in
-  let f = c +% g in
-  let x3 = e *% f in
-  let y3 = g *% h in
-  let t3 = e *% h in
-  let z3 = f *% g in
-  (x3, y3, z3, t3)
+let aff_point_c = p:aff_point{is_on_curve p}
+let aff_point_add_c (p:aff_point_c) (q:aff_point_c) : aff_point_c =
+  EL.aff_point_add_lemma p q;
+  aff_point_add p q
 
-let ith_bit (k:lbytes 32) (i:size_nat{i < 256}) =
-  let q = i / 8 in let r = size (i % 8) in
-  (index #uint8 #32 k q >>. r) &. u8 1
+let mk_ed25519_comm_monoid: LE.comm_monoid aff_point_c = {
+  LE.one = aff_point_at_infinity;
+  LE.mul = aff_point_add_c;
+  LE.lemma_one = EL.aff_point_at_infinity_lemma;
+  LE.lemma_mul_assoc = EL.aff_point_add_assoc_lemma;
+  LE.lemma_mul_comm = EL.aff_point_add_comm_lemma;
+  }
 
-let cswap2 (sw:uint8) (x:ext_point) (xp1:ext_point) =
-  if uint_to_nat sw = 1 then (xp1, x) else (x, xp1)
+let ext_point_c = p:ext_point{is_ext p /\ is_on_curve (to_aff_point p)}
+let mk_to_ed25519_comm_monoid : SE.to_comm_monoid ext_point_c = {
+  SE.a_spec = aff_point_c;
+  SE.comm_monoid = mk_ed25519_comm_monoid;
+  SE.refl = (fun (x:ext_point_c) -> to_aff_point x);
+  }
 
-let ladder_step (k:lbytes 32) (i:nat{i < 256}) (x, xp1) =
-  let bit = ith_bit k (255 - i) in
-  let x, xp1 = cswap2 bit x xp1 in
-  let xx = point_double x in
-  let xxp1 = point_add x xp1 in
-  cswap2 bit xx xxp1
+val point_at_inifinity_c: SE.one_st ext_point_c mk_to_ed25519_comm_monoid
+let point_at_inifinity_c _ =
+  EL.to_aff_point_at_infinity_lemma ();
+  point_at_infinity
 
-let montgomery_ladder (x:ext_point) (xp1:ext_point) (k:lbytes 32) : Tot (ext_point & ext_point) =
-  Lib.LoopCombinators.repeati 256 (ladder_step k) (x, xp1)
+val point_add_c: SE.mul_st ext_point_c mk_to_ed25519_comm_monoid
+let point_add_c p q =
+  let r = point_add p q in
+  EL.to_aff_point_add_lemma p q;
+  EL.aff_point_add_lemma (to_aff_point p) (to_aff_point q);
+  r
 
-let point_mul (a:lbytes 32) (p:ext_point) =
-  fst (montgomery_ladder (zero, one, one, zero) p a)
+val point_double_c: SE.sqr_st ext_point_c mk_to_ed25519_comm_monoid
+let point_double_c p =
+  let r = point_double p in
+  EL.to_aff_point_double_lemma p;
+  EL.aff_point_double_lemma (to_aff_point p);
+  EL.aff_point_add_lemma (to_aff_point p) (to_aff_point p);
+  r
 
-let recover_x (y:nat) (sign:bool) : Tot (option elem) =
-  if y >= prime then None
-  else (
-    let y2 = y *% y in
-    let x2 = (y2 -% one) *% (modp_inv ((d *% y2) +% one)) in
-    if x2 = zero then (
-      if sign then None
-      else Some zero)
-    else (
-      let x = x2 **% ((prime + 3) / 8) in
-      let x = if ((x *% x) -% x2) <> zero then x *% modp_sqrt_m1 else x in
-      if ((x *% x) -% x2) <> zero then None
-      else (
-        let x = if (x % 2 = 1) <> sign then (prime - x) % prime else x in
-        Some x)))
+let mk_ed25519_concrete_ops : SE.concrete_ops ext_point_c = {
+  SE.to = mk_to_ed25519_comm_monoid;
+  SE.one = point_at_inifinity_c;
+  SE.mul = point_add_c;
+  SE.sqr = point_double_c;
+  }
 
-let point_compress (p:ext_point) : Tot (lbytes 32) =
-  let px, py, pz, pt = p in
-  let zinv = modp_inv pz in
-  let x = px *% zinv in
-  let y = py *% zinv in
-  nat_to_bytes_le 32 (pow2 255 * (x % 2) + y)
+let point_mul (a:lbytes 32) (p:ext_point_c) : ext_point_c =
+  SE.exp_fw mk_ed25519_concrete_ops p 256 (nat_from_bytes_le a) 4
 
-let point_decompress (s:lbytes 32) : Tot (option ext_point) =
-  let y = nat_from_bytes_le s in
-  let sign = (y / pow2 255) % 2 = 1 in
-  let y = y % pow2 255 in
-  let x = recover_x y sign in
-  match x with
-  | Some x -> Some (x, y, one, x *% y)
-  | _ -> None
+let point_mul_double (a1:lbytes 32) (p1:ext_point_c) (a2:lbytes 32) (p2:ext_point_c) : ext_point_c =
+  SE.exp_double_fw mk_ed25519_concrete_ops p1 256 (nat_from_bytes_le a1) p2 (nat_from_bytes_le a2) 4
+
+let point_mul_g (a:lbytes 32) : ext_point_c =
+  EL.g_is_on_curve ();
+  point_mul a g
+
+let point_mul_double_g (a1:lbytes 32) (a2:lbytes 32) (p:ext_point_c) : ext_point_c =
+  EL.g_is_on_curve ();
+  point_mul_double a1 g a2 p
+
+
+///  Ed25519 API
 
 let secret_expand (secret:lbytes 32) : (lbytes 32 & lbytes 32) =
   let h = Spec.Agile.Hash.hash Spec.Hash.Definitions.SHA2_512 secret in
@@ -143,36 +104,29 @@ let secret_expand (secret:lbytes 32) : (lbytes 32 & lbytes 32) =
   let h_low = h_low.[31] <- (index #uint8 #32 h_low 31 &. u8 127) |. u8 64 in
   h_low, h_high
 
+
 let secret_to_public (secret:lbytes 32) =
   let a, dummy = secret_expand secret in
-  point_compress (point_mul a g)
+  point_compress (point_mul_g a)
 
-let point_equal (p:ext_point) (q:ext_point) =
-  let px, py, pz, pt = p in
-  let qx, qy, qz, qt = q in
-  if ((px *% qz) <> (qx *% pz)) then false
-  else if ((py *% qz) <> (qy *% pz)) then false
-  else true
 
-///
-/// Ed25519 API
-///
-
-let expand_keys (secret: lbytes 32) : (lbytes 32 & lbytes 32 & lbytes 32) =
+let expand_keys (secret:lbytes 32) : (lbytes 32 & lbytes 32 & lbytes 32) =
   let s, prefix = secret_expand secret in
   let pub = secret_to_public secret in
   pub, s, prefix
 
+
 val sign_expanded:
-  pub:lbytes 32 ->
-  s:lbytes 32 ->
-  prefix:lbytes 32 ->
-  msg: bytes{64 + length msg <= max_size_t} ->
-  Tot (lbytes 64)
+    pub:lbytes 32
+  -> s:lbytes 32
+  -> prefix:lbytes 32
+  -> msg:bytes{64 + length msg <= max_size_t} ->
+  lbytes 64
+
 let sign_expanded pub s prefix msg =
   let len = length msg in
   let r = sha512_modq (32 + len) (concat #uint8 #32 #(length msg) prefix msg) in
-  let r' = point_mul (nat_to_bytes_le 32 r) g in
+  let r' = point_mul_g (nat_to_bytes_le 32 r) in
   let rs = point_compress r' in
   let h = sha512_modq (64 + len)
     (concat #uint8 #64 #(length msg) (concat #uint8 #32 #32 rs pub) msg)
@@ -180,20 +134,18 @@ let sign_expanded pub s prefix msg =
   let s = (r + (h * nat_from_bytes_le s) % q) % q in
   concat #uint8 #32 #32 rs (nat_to_bytes_le 32 s)
 
-val sign:
-    secret: lbytes 32
-  -> msg: bytes{64 + length msg <= max_size_t} ->
-  Tot (lbytes 64)
 
+val sign: secret:lbytes 32 -> msg:bytes{64 + length msg <= max_size_t} -> lbytes 64
 let sign secret msg =
   let pub, s, prefix = expand_keys secret in
   sign_expanded pub s prefix msg
 
+
 val verify:
-    public: lbytes 32
-  -> msg: bytes{64 + length msg <= max_size_t}
-  -> signature: lbytes 64 ->
-  Tot bool
+    public:lbytes 32
+  -> msg:bytes{64 + length msg <= max_size_t}
+  -> signature:lbytes 64 ->
+  bool
 
 let verify public msg signature =
   let len = length msg in
@@ -212,9 +164,13 @@ let verify public msg signature =
         let h = sha512_modq (64 + len)
 	  (concat #uint8 #64 #(length msg) (concat #uint8 #32 #32 rs public) msg)
 	in
-        let sB = point_mul (nat_to_bytes_le 32 s) g in
-        let hA = point_mul (nat_to_bytes_le 32 h) a' in
-        point_equal sB (point_add r' hA)
+        let sb = nat_to_bytes_le 32 s in
+        let hb = nat_to_bytes_le 32 h in
+        let a'' = point_negate a' in
+
+        EL.point_negate_decompress_lemma public;
+        let exp_d = point_mul_double_g sb hb a'' in
+        point_equal exp_d r'
       )
     )
   )
